Foundation/Modal/Boxdot/Jerabek.lean
@@ -61,7 +61,7 @@ def Frame.twice.PMorphism (F : Frame) : F×2 →ₚ F where
   toFun := Prod.fst
   forth := by
     rintro ⟨x, _⟩ ⟨y, _⟩ h;
-    simpa using h;
+    simpa using! h;
   back := by
     intro ⟨x, i⟩ y Rxy;
     use ⟨y, true⟩;
@@ -228,15 +228,15 @@ theorem jerabek_SBDP
   let X := X₀ ∪ X₁;
   let XB := X.image (·ᵇ);
 
-  have Claim1 : ∀ ψ ∈ (□⁻¹'φ.subformulas), (L, XB.toSet) ⊢ □ψᵇ 🡒 ψᵇ := by
+  have Claim1 : ∀ ψ ∈ (□⁻¹'φ.subformulas), (L, (↑XB : Set (Formula ℕ))) ⊢ □ψᵇ 🡒 ψᵇ := by
     intro ψ hψ;
-    have H₁ : ∀ b, (L, XB.toSet) ⊢ (flag (.atom q) b) ⋏ □ψᵇ 🡒 ⊡((flag (.atom q) !b) 🡒 ψᵇ) := by
+    have H₁ : ∀ b, (L, (↑XB : Set (Formula ℕ))) ⊢ (flag (.atom q) b) ⋏ □ψᵇ 🡒 ⊡((flag (.atom q) !b) 🡒 ψᵇ) := by
       intro b;
       apply GlobalConsequence.thm!;
       apply jerabek_SBDP.lemma₂;
-    have H₂ : ∀ b, (L, XB.toSet) ⊢ ⊡((flag (.atom q) b) 🡒 ψᵇ) 🡒 ψᵇ := by
+    have H₂ : ∀ b, (L, (↑XB : Set (Formula ℕ))) ⊢ ⊡((flag (.atom q) b) 🡒 ψᵇ) 🡒 ψᵇ := by
       intro b;
-      suffices (L, XB.toSet) ⊢ (□((flag (.atom q) b) 🡒 ψ) 🡒 ψ)ᵇ by
+      suffices (L, (↑XB : Set (Formula ℕ))) ⊢ (□((flag (.atom q) b) 🡒 ψ) 🡒 ψ)ᵇ by
         simpa only [Formula.boxdotTranslate, Formula.atom_flag_boxdotTranslated] using this;
       apply GlobalConsequence.ctx!;
       simp only [Finset.coe_image, Set.mem_image, Finset.mem_coe, XB];
@@ -248,13 +248,13 @@ theorem jerabek_SBDP
           simp [X, X₀, X₁, flag, Finset.LO.preboxItr];
           grind;
       . rfl;
-    have H₃ : ∀ b, (L, XB.toSet) ⊢ (flag (.atom q) b) 🡒 (□ψᵇ 🡒 ψᵇ) := by
+    have H₃ : ∀ b, (L, (↑XB : Set (Formula ℕ))) ⊢ (flag (.atom q) b) 🡒 (□ψᵇ 🡒 ψᵇ) := by
       intro b;
       cl_prover [(H₁ b), (H₂ !b)];
-    have H₄ : (L, XB.toSet) ⊢  atom q 🡒 □ψᵇ 🡒 ψᵇ := H₃ true;
-    have H₅ : (L, XB.toSet) ⊢ ∼atom q 🡒 □ψᵇ 🡒 ψᵇ := H₃ false;
+    have H₄ : (L, (↑XB : Set (Formula ℕ))) ⊢  atom q 🡒 □ψᵇ 🡒 ψᵇ := H₃ true;
+    have H₅ : (L, (↑XB : Set (Formula ℕ))) ⊢ ∼atom q 🡒 □ψᵇ 🡒 ψᵇ := H₃ false;
     cl_prover [H₄, H₅];
-  have Claim2 : ∀ ψ ∈ φ.subformulas, (L, XB.toSet) ⊢ ψ 🡘 ψᵇ := by
+  have Claim2 : ∀ ψ ∈ φ.subformulas, (L, (↑XB : Set (Formula ℕ))) ⊢ ψ 🡘 ψᵇ := by
     intro ψ hψ;
     induction ψ with
     | hfalsum => simp [Formula.boxdotTranslate];
@@ -265,17 +265,17 @@ theorem jerabek_SBDP
       dsimp [Formula.boxdotTranslate];
       cl_prover [ihψ₁, ihψ₂];
     | hbox ψ ihψ =>
-      replace ihψ : (L, XB.toSet) ⊢ ψ 🡘 ψᵇ := ihψ (by grind);
-      have H₁ : (L, XB.toSet) ⊢ □ψ 🡘 □ψᵇ := box_congruence! ihψ;
-      have H₂ : (L, XB.toSet) ⊢ □ψᵇ 🡘 ⊡ψᵇ := by
+      replace ihψ : (L, (↑XB : Set (Formula ℕ))) ⊢ ψ 🡘 ψᵇ := ihψ (by grind);
+      have H₁ : (L, (↑XB : Set (Formula ℕ))) ⊢ □ψ 🡘 □ψᵇ := box_congruence! ihψ;
+      have H₂ : (L, (↑XB : Set (Formula ℕ))) ⊢ □ψᵇ 🡘 ⊡ψᵇ := by
         apply Entailment.E!_intro;
-        . have : (L, XB.toSet) ⊢ □ψᵇ 🡒 ψᵇ := Claim1 ψ (by simpa [Finset.LO.preboxItr]);
+        . have : (L, (↑XB : Set (Formula ℕ))) ⊢ □ψᵇ 🡒 ψᵇ := Claim1 ψ (by simpa [Finset.LO.preboxItr]);
           cl_prover [this];
         . cl_prover;
       cl_prover [H₁, H₂];
-  have : (L, XB.toSet) ⊢ φᵇ := by
-    have h₁ : (L, XB.toSet) ⊢ φ 🡒 φᵇ := C_of_E_mp! $ Claim2 φ (by grind);
-    have h₂ : (L, XB.toSet) ⊢ φ := by
+  have : (L, (↑XB : Set (Formula ℕ))) ⊢ φᵇ := by
+    have h₁ : (L, (↑XB : Set (Formula ℕ))) ⊢ φ 🡒 φᵇ := C_of_E_mp! $ Claim2 φ (by grind);
+    have h₂ : (L, (↑XB : Set (Formula ℕ))) ⊢ φ := by
       apply GlobalConsequence.thm!;
       grind;
     exact h₁ ⨀ h₂;
