Foundation/Modal/Kripke/Logic/GrzPoint2.lean
@@ -71,7 +71,7 @@ open LO.Entailment LO.Entailment.FiniteContext LO.Modal.Entailment
 
 instance : Modal.Grz ⪯ Modal.GrzPoint2 := Hilbert.Normal.weakerThan_of_subset_axioms $ by grind;
 
-lemma GrzPoint2_of_Grz (h : (φ.atoms.image (λ a => Axioms.Point2 (.atom a))).toSet *⊢[Modal.Grz] φ) : Modal.GrzPoint2 ⊢ φ := by
+lemma GrzPoint2_of_Grz (h : (↑(φ.atoms.image (λ a => Axioms.Point2 (Formula.atom a))) : Set (Formula ℕ)) *⊢[Modal.Grz] φ) : Modal.GrzPoint2 ⊢ φ := by
   obtain ⟨Γ, hΓ₁, hΓ₂⟩ := Context.provable_iff.mp h;
   simp only [Finset.coe_image, Set.mem_image, Finset.mem_coe] at hΓ₁;
   replace hΓ₂ : Modal.GrzPoint2 ⊢ ⋀Γ 🡒 φ := WeakerThan.pbl $ FiniteContext.provable_iff.mp hΓ₂;
