Foundation/Modal/Tableau.lean
@@ -782,7 +782,7 @@ private lemma of_mem₂_boxItr : (□^[n]φ ∈ t.1.2) → (∃ t' : MaximalCons
     . rintro ψ hψ;
       obtain ⟨ξ, hξ, rfl⟩ := Finset.LO.exists_of_mem_boxItr hψ;
       simp at hΓ;
-      simpa using hΓ $ by simpa;
+      exact hΓ $ by simpa;
     . simpa;
   use t';
   constructor;
